categorical composition preserves simulation

common/CategoricalComp.v
@@ -1,10 +1,11 @@
 Require Import Relations.
 Require Import List.
 Require Import Coqlib.
-Require Import LanguageInterface.
+Require Import LanguageInterface_.
 Require Import Events.
 Require Import Globalenvs.
 Require Import SmallstepLinking.
+Require Import Smallstep.
 Require Import Smallstep_.
 Require Import Integers.
 Require Import Linking.
@@ -19,7 +20,7 @@ Section COMP.
   Let L1 := Lsem1 se.
   Let Li1 := Lsem1 se qset.
   Let L2 := Lsem2 se.
-  Let Li2 := Lsem2 se (fun i => footprint L1 i \/ qset i).
+  Let Li2 := Lsem2 se (fun i => footprint Lsem1 i \/ qset i).
 
   Definition valid_query' {li} (q: query li): Prop :=
     exists i, qset i /\ Genv.symbol_address se i Ptrofs.zero = entry q.
@@ -37,7 +38,7 @@ Section COMP.
   | step_push s1 q s2:
       at_external L1 s1 q ->
       initial_state L2 q s2 ->
-      not (valid_query L1 se q) ->
+      not (valid_query Lsem1 se q) ->
       not (valid_query' q) ->
       comp_step (st1 s1) E0 (st2 s1 s2)
   | step_pop s1 r s2 s1':
@@ -52,8 +53,8 @@ Section COMP.
 
   Inductive comp_at_external: comp_state -> query liA -> Prop :=
   | comp_at_external_intro s1 s2 (q: query liA):
-      not (valid_query L1 se q) ->
-      not (valid_query L2 se q) ->
+      not (valid_query Lsem1 se q) ->
+      not (valid_query Lsem2 se q) ->
       at_external L2 s2 q ->
       comp_at_external (st2 s1 s2) q.
 
@@ -74,12 +75,42 @@ Section COMP.
     |}.
   Definition comp_lts_external :=
     {|
-    footprint i := footprint L1 i \/ footprint L2 i;
     initial_state := comp_initial_state;
     at_external := comp_at_external;
     after_external := comp_after_external;
     final_state := comp_final_state;
     |}.
+
+  Lemma star_internal1 s t s':
+    Star Li1 s t s' ->
+    star (fun _ => comp_step) tt (st1 s) t (st1 s').
+  Proof.
+    induction 1; [eapply star_refl | eapply star_step]; eauto.
+    constructor; auto.
+  Qed.
+
+  Lemma plus_internal1 s t s':
+    Plus Li1 s t s' ->
+    plus (fun _ => comp_step) tt (st1 s) t (st1 s').
+  Proof.
+    destruct 1; econstructor; eauto using step1, star_internal1.
+  Qed.
+
+  Lemma star_internal2 s1 s t s':
+    Star Li2 s t s' ->
+    star (fun _ => comp_step) tt (st2 s1 s) t (st2 s1 s').
+  Proof.
+    induction 1; [eapply star_refl | eapply star_step]; eauto.
+    constructor; auto.
+  Qed.
+
+  Lemma plus_internal2 s1 s t s':
+    Plus Li2 s t s' ->
+    plus (fun _ => comp_step) tt (st2 s1 s) t (st2 s1 s').
+  Proof.
+    destruct 1; econstructor; eauto using step2, star_internal2.
+  Qed.
+
 End COMP.
 
 Definition comp_semantics' {liA liB liC} (L1: semantics liB liC)
@@ -90,7 +121,8 @@ Definition comp_semantics' {liA liB liC} (L1: semantics liB liC)
       steps p := comp_lts_internal L1 L2 se p;
       events := comp_lts_external L1 L2 se;
     |};
-    skel := sk;
+  skel := sk;
+  footprint i := footprint L1 i \/ footprint L2 i;
   |}.
 
 Definition comp_semantics {liA liB liC} (L1: semantics liB liC)
@@ -234,93 +266,97 @@ Section ASSOC.
   (* Lemma assoc1: L1 ∘ (L2 ∘ L3) ≤ L1 ∘ L2 ∘ L3. *)
   Lemma assoc1: L' ≤ L.
   Proof.
-    constructor. econstructor. reflexivity.
-    intros se _ [ ] qset [ ] Hse.
-    instantiate (1 := fun _ _ _ => _). cbn beta.
-    apply forward_simulation_step
-      with (match_states := assoc_state_match); cbn.
-    - intros. now rewrite or_assoc.
-    - intros q _ s1 [ ] H. inv H.
-      eexists. split; try repeat constructor; auto.
-    - intros s1 s2 r Hs H. inv H. inv Hs.
-      eexists. split; try repeat constructor; auto.
-    - intros s1 s2 q Hs Hext. inv Hext. inv H1. inv Hs.
-      eexists tt, _. repeat apply conj; try repeat constructor; auto.
-      intros [i [[Hi1 | Hi2] ?]];
-        [ apply H; eexists; split; eauto |
-          apply H2; eexists; split; eauto ].
-      intros r _ s1' [ ] Haft. inv Haft. inv H8.
-      eexists. split; try repeat constructor; auto.
-    - intros s1 t s1' Hstep s2 Hs.
-      inv Hstep.
-      + inv Hs. eexists; split; try repeat constructor; auto.
-      + inv H; inv Hs; eexists; (split; [ | constructor ]).
-        * apply step1. now apply step2.
-        * apply step2. eapply qset_step. eauto.
-          apply functional_extensionality. intros x.
-          apply EquivThenEqual.
-          cbn. rewrite <- or_assoc. apply or_iff_compat_r.
-          apply or_comm.
-        * (* eapply step_push; try constructor; eauto. *)
-          eapply step_push; eauto.
-          constructor; auto.
-          -- intros [x [? ?]]. apply H3. eexists; split; eauto.
-          -- intros [x [[? | ?] ?]].
-             apply H3. eexists; split; eauto.
-             apply H2. eexists; split; eauto.
-          -- intros [x [? ?]]. apply H3. eexists; split; eauto.
-        * eapply step_pop; try constructor; eauto.
-      + inv H0. eexists; split; [ | constructor ].
-        inv Hs. constructor. eapply step_push; eauto.
-      + inv H. eexists; split; [ | constructor].
-        inv Hs. constructor. econstructor; eauto.
+    constructor. econstructor.
+    - reflexivity.
+    - intros. cbn. now rewrite or_assoc.
+    - { intros se _ [ ] qset [ ] Hse.
+        instantiate (1 := fun _ _ _ => _). cbn beta.
+        apply forward_simulation_step
+          with (match_states := assoc_state_match); cbn.
+        - intros q _ s1 [ ] H. inv H.
+          eexists. split; try repeat constructor; auto.
+        - intros s1 s2 r Hs H. inv H. inv Hs.
+          eexists. split; try repeat constructor; auto.
+        - intros s1 s2 q Hs Hext. inv Hext. inv H1. inv Hs.
+          eexists tt, _. repeat apply conj; try repeat constructor; auto.
+          intros [i [[Hi1 | Hi2] ?]];
+            [ apply H; eexists; split; eauto |
+              apply H2; eexists; split; eauto ].
+          intros r _ s1' [ ] Haft. inv Haft. inv H8.
+          eexists. split; try repeat constructor; auto.
+        - intros s1 t s1' Hstep s2 Hs.
+          inv Hstep.
+          + inv Hs. eexists; split; try repeat constructor; auto.
+          + inv H; inv Hs; eexists; (split; [ | constructor ]).
+            * apply step1. now apply step2.
+            * apply step2. eapply qset_step. eauto.
+              apply functional_extensionality. intros x.
+              apply EquivThenEqual.
+              cbn. rewrite <- or_assoc. apply or_iff_compat_r.
+              apply or_comm.
+            * (* eapply step_push; try constructor; eauto. *)
+              eapply step_push; eauto.
+              constructor; auto.
+              -- intros [x [? ?]]. apply H3. eexists; split; eauto.
+              -- intros [x [[? | ?] ?]].
+                 apply H3. eexists; split; eauto.
+                 apply H2. eexists; split; eauto.
+              -- intros [x [? ?]]. apply H3. eexists; split; eauto.
+            * eapply step_pop; try constructor; eauto.
+          + inv H0. eexists; split; [ | constructor ].
+            inv Hs. constructor. eapply step_push; eauto.
+          + inv H. eexists; split; [ | constructor].
+            inv Hs. constructor. econstructor; eauto.
+      }
     - apply well_founded_ltof.
   Qed.
 
   (* Lemma assoc2: L1 ∘ L2 ∘ L3 ≤ L1 ∘ (L2 ∘ L3). *)
   Lemma assoc2: L ≤ L'.
   Proof.
-    constructor. econstructor. reflexivity.
-    intros se _ [ ] qset [ ] Hse.
-    instantiate (1 := fun _ _ _ => _). cbn beta.
-    apply forward_simulation_step
-      with (match_states := fun s1 s2 => assoc_state_match s2 s1); cbn.
-    - intros i. now rewrite or_assoc.
-    - intros q _ s1 [ ] H. inv H. inv H0.
-      eexists; split; constructor; auto.
-    - intros s1 s2 r Hs H. inv H. inv H0. inv Hs.
-      eexists; split; constructor; auto.
-    - intros s1 s2 q Hs Hext. inv Hext. inv Hs.
-      eexists tt, _. repeat apply conj; try repeat constructor; auto.
-      + intros [x [? ?]]. apply H. eexists; split; eauto.
-        left; auto.
-      + intros [x [[|]]].
-        apply H. eexists; split; eauto. right. auto.
-        apply H0. eexists; split; eauto.
-      + intros [x [? ?]].  apply H. eexists; split; eauto.
-        right; auto.
-      + intros r _ s1' [ ] Haft. inv Haft.
-        eexists; split; repeat constructor; auto.
-    - intros s1 t s1' Hstep s2 Hs.
-      inv Hstep.
-      + inv H; inv Hs; eexists; (split; [ | constructor ]).
-        * now apply step1.
-        * apply step2. now apply step1.
-        * eapply step_push; try constructor; eauto.
-        * eapply step_pop; try constructor; eauto.
-      + inv Hs. eexists; split; repeat constructor; auto.
-        eapply qset_step. eauto.
-        apply functional_extensionality. intros x.
-        apply EquivThenEqual.
-        cbn. rewrite <- or_assoc. apply or_iff_compat_r.
-        apply or_comm.
-      + inv H. inv Hs. eexists; split; constructor.
-        eapply step_push; eauto.
-        intros [x [[|]]].
-        apply H3. eexists; split; eauto.
-        apply H2. eexists; split; eauto.
-      + inv H0. inv Hs. eexists; split; constructor.
-        eapply step_pop; eauto.
+    constructor. econstructor.
+    - reflexivity.
+    - intros. cbn. now rewrite or_assoc.
+    - { intros se _ [ ] qset [ ] Hse.
+        instantiate (1 := fun _ _ _ => _). cbn beta.
+        apply forward_simulation_step
+          with (match_states := fun s1 s2 => assoc_state_match s2 s1); cbn.
+        - intros q _ s1 [ ] H. inv H. inv H0.
+          eexists; split; constructor; auto.
+        - intros s1 s2 r Hs H. inv H. inv H0. inv Hs.
+          eexists; split; constructor; auto.
+        - intros s1 s2 q Hs Hext. inv Hext. inv Hs.
+          eexists tt, _. repeat apply conj; try repeat constructor; auto.
+          + intros [x [? ?]]. apply H. eexists; split; eauto.
+            left; auto.
+          + intros [x [[|]]].
+            apply H. eexists; split; eauto. right. auto.
+            apply H0. eexists; split; eauto.
+          + intros [x [? ?]].  apply H. eexists; split; eauto.
+            right; auto.
+          + intros r _ s1' [ ] Haft. inv Haft.
+            eexists; split; repeat constructor; auto.
+        - intros s1 t s1' Hstep s2 Hs.
+          inv Hstep.
+          + inv H; inv Hs; eexists; (split; [ | constructor ]).
+            * now apply step1.
+            * apply step2. now apply step1.
+            * eapply step_push; try constructor; eauto.
+            * eapply step_pop; try constructor; eauto.
+          + inv Hs. eexists; split; repeat constructor; auto.
+            eapply qset_step. eauto.
+            apply functional_extensionality. intros x.
+            apply EquivThenEqual.
+            cbn. rewrite <- or_assoc. apply or_iff_compat_r.
+            apply or_comm.
+          + inv H. inv Hs. eexists; split; constructor.
+            eapply step_push; eauto.
+            intros [x [[|]]].
+            apply H3. eexists; split; eauto.
+            apply H2. eexists; split; eauto.
+          + inv H0. inv Hs. eexists; split; constructor.
+            eapply step_pop; eauto.
+      }
     - apply well_founded_ltof.
   Qed.
 
@@ -343,24 +379,30 @@ Section FSIM.
           (se1 se2: Genv.symtbl) (w : ccworld cc3) (qset: ident -> Prop)
           (Hse: match_senv cc3 w se1 se2)
           (Hse1: Genv.valid_for (skel L1) se1)
-          (Hse2: Genv.valid_for (skel L1') se1).
+          (Hse2: Genv.valid_for (skel L2) se1).
 
   Variant index := | index1: fsim_index HL1 -> index
-  | index2: fsim_index HL1 -> fsim_index HL2 -> index.
+                   | index2: fsim_index HL1 -> fsim_index HL2 -> index.
 
   Variant order: index -> index -> Prop :=
   | order1 i1 i1': fsim_order HL1 i1 i1' ->
-      order (index1 i1) (index1 i1')
-  | order2 i1 i1' i2 i2': fsim_order HL2 i2 i2' ->
-      order (index2 i1 i2) (index2 i1' i2').
+                   order (index1 i1) (index1 i1')
+  | order2 i1 i2 i2': fsim_order HL2 i2 i2' ->
+                      order (index2 i1 i2) (index2 i1 i2').
 
   Inductive match_states: index -> comp_state L1 L2 -> comp_state L1' L2' -> Prop :=
   | match_st1 i1 s1 s1':
       fsim_match_states HL1 se1 se2 w i1 s1 s1' ->
       match_states (index1 i1) (st1 L1 L2 s1) (st1 L1' L2' s1')
   | match_st2 i1 i2 s1 s1' s2 s2' w':
-      fsim_match_states HL1 se1 se2 w i1 s1 s1' ->
+      match_senv cc2 w' se1 se2 ->
       fsim_match_states HL2 se1 se2 w' i2 s2 s2' ->
+      (forall r1 r2 (s2 : state L1),
+          match_reply cc2 w' r1 r2 ->
+          after_external (L1 se1) s1 r1 s2 ->
+          exists (i' : fsim_index HL1) (s2' : state L1'),
+            after_external (L1' se2) s1' r2 s2' /\
+            fsim_match_states HL1 se1 se2 w i' s2 s2') ->
       match_states (index2 i1 i2) (st2 L1 L2 s1 s2) (st2 L1' L2' s1' s2').
 
   Lemma comp_semantics_simulation sk sk':
@@ -370,9 +412,106 @@ Section FSIM.
                     index order match_states.
   Proof.
     split; cbn.
-  Admitted.
+    - intros q1 q2 s1 Hq H. inv H.
+      pose proof (fsim_lts HL1 _ _ qset Hse Hse1).
+      edestruct @fsim_match_initial_states as (idx & s' & Hs' & Hs); eauto.
+      exists (index1 idx), (st1 L1' L2' s'). split; econstructor; eauto.
+    - intros i s1 s2 r1 Hs H. inv H. inv Hs.
+      pose proof (fsim_lts HL1 _ _ qset Hse Hse1).
+      edestruct @fsim_match_final_states as (r' & H' & Hr'); eauto.
+      exists r'. split; auto. constructor; auto.
+    - intros i s1 s2 q1 Hs H. inv H. inv Hs.
+      pose proof (fsim_lts HL2 _ _ qset H4 Hse2).
+      edestruct @fsim_match_external as (w1 & q' & H' & Hq' & Hse' & HH); eauto.
+      exists w1, q'. repeat apply conj; auto.
+      + constructor; auto.
+        erewrite <- match_valid_query; [ | constructor; apply HL1 | .. ]; eauto.
+        erewrite <- match_valid_query; [ | constructor; apply HL2 | .. ]; eauto.
+      + intros r1 r2 xs1 Hr HH'. inv HH'.
+        specialize (HH _ _ _ Hr H10) as (i2' & xs2 & Haft & Hss).
+        eexists (index2 i1 i2'), (st2 L1' L2' _ _). split.
+        * econstructor. eauto.
+        * econstructor; eauto.
+    - intros s1 t s2 Hstep idx s1' Hs.
+      inv Hstep; inv Hs.
+      + pose proof (fsim_lts HL1 _ _ qset Hse Hse1).
+        edestruct @fsim_simulation as (idx' & s2' & Hs2' & Hs'); eauto.
+        exists (index1 idx'), (st1 L1' L2' s2'). split.
+        * destruct Hs2'; [ left | right ].
+          apply plus_internal1. auto.
+          split. apply star_internal1. apply H1. constructor; apply H1.
+        * constructor. auto.
+      + pose proof (fsim_lts HL2 _ _ (fun i => footprint L1 i \/ qset i) H2 Hse2).
+        edestruct @fsim_simulation as (idx' & xs2' & Hs2' & Hs'); eauto.
+        exists (index2 i1 idx'), (st2 L1' L2' s1'0 xs2'). split.
+        * destruct Hs2'; [ left | right ].
+          -- apply plus_internal2.
+             replace (fun i : ident => footprint L1' i \/ qset i) with
+                 (fun i : ident => footprint L1 i \/ qset i); auto.
+             apply functional_extensionality. intros x.
+             apply EquivThenEqual.
+             apply or_iff_compat_r.
+             eapply fsim_footprint. eauto.
+          -- split. apply star_internal2.
+             destruct H1.
+             replace (fun i : ident => footprint L1' i \/ qset i) with
+                 (fun i : ident => footprint L1 i \/ qset i); auto.
+             apply functional_extensionality. intros x.
+             apply EquivThenEqual.
+             apply or_iff_compat_r.
+             eapply fsim_footprint. eauto.
+             constructor. apply H1.
+        * econstructor; eauto.
+      + pose proof (fsim_lts HL1 _ _ qset Hse Hse1).
+        edestruct @fsim_match_external as (w' & q' & H' & Hq' & Hse' & HH); eauto.
+        pose proof (fsim_lts HL2 _ _ (fun i => footprint L1 i \/ qset i) Hse' Hse2).
+        edestruct @fsim_match_initial_states as (i2 & s2' & Hs2' & Hs'); eauto.
+        exists (index2 i1 i2), (st2 L1' L2' s1'0 s2'). split.
+        * left. apply plus_one. eapply step_push; eauto.
+          erewrite <- match_valid_query; [ | constructor; apply HL1 | .. ]; eauto.
+          intros [i [Hi Hix]]. apply H2. exists i. split; auto.
+          erewrite match_senv_symbol_address; eauto.
+        * econstructor; eauto.
+      + pose proof (fsim_lts HL2 _ _ (fun i => footprint L1 i \/ qset i) H3 Hse2).
+        edestruct @fsim_match_final_states as (r' & H' & Hr'); eauto.
+        edestruct H7 as (idx & xs2' & HH & Hs2'); eauto.
+        exists (index1 idx), (st1 L1' L2' xs2'). split.
+        * left. apply plus_one. eapply step_pop; eauto.
+        * constructor. auto.
+  Qed.
 
 End FSIM.
+
+Lemma categorical_comp_simulation
+      {liA1 liA2 liB1 liB2 liC1 liC2}
+      (cc1: callconv liA1 liA2) (cc2: callconv liB1 liB2) (cc3: callconv liC1 liC2)
+      L1a L1b L1 L2a L2b L2:
+  forward_simulation cc2 cc3 L1a L2a ->
+  forward_simulation cc1 cc2 L1b L2b ->
+  L1a ∘ L1b = Some L1 -> L2a ∘ L2b = Some L2 ->
+  forward_simulation cc1 cc3 L1 L2.
+Proof.
+  intros [Ha] [Hb] H1 H2. unfold comp_semantics in *. unfold option_map in *.
+  destruct (link (skel L1a) (skel L1b)) as [sk1|] eqn:Hsk1; try discriminate. inv H1.
+  destruct (link (skel L2a) (skel L2b)) as [sk2|] eqn:Hsk2; try discriminate. inv H2.
+  constructor.
+  eapply Forward_simulation
+    with (order cc1 cc2 cc3 L1a L1b L2a L2b Ha Hb)
+         (match_states cc1 cc2 cc3 L1a L1b L2a L2b Ha Hb).
+  - cbn. destruct Ha, Hb. congruence.
+  - cbn. intros i. destruct Ha, Hb.
+    rewrite fsim_footprint, fsim_footprint0. reflexivity.
+  - intros se1 se2 w qset Hse Hse1.
+    pose proof (link_linkorder _ _ _ Hsk1) as [Hsk1a Hsk1b].
+    eapply comp_semantics_simulation; eauto.
+    eapply Genv.valid_for_linkorder; eauto.
+    eapply Genv.valid_for_linkorder; eauto.
+  - clear - Ha Hb. intros [|].
+    + induction (fsim_order_wf Ha f). constructor.
+      intros. inv H1. apply H0. auto.
+    + induction (fsim_order_wf Hb f0). constructor.
+      intros. inv H1. apply H0. auto.
+Qed.
 
 Section APPROX.
   Context {liA liB liC} (L1: semantics liB liC) (L2: semantics liA liB).
